ML_SP_Definitions.v
@@ -306,6 +306,7 @@ Definition env_fv :=
 
 Module Type DeltaIntf.
   Parameter type : Const.const -> sch.
+  Parameter closed : forall c, sch_fv (type c) = {}.
   Parameter rule : nat -> trm -> trm -> Prop.
   Parameter term : forall n t1 t2 tl,
     rule n t1 t2 ->
